src/Sound/Semantics/Omni.dfy
@@ -1,12 +1,17 @@
 module Omni {
   import opened Defs
   export
-    provides Defs, SeqLemma, SeqChoiceLemma
-    reveals Sem, SeqSem, VarDeclWitness
+    provides Defs, SeqLemma, SemNest, WP, SemCons, SeqFrameLemmaAll
+    reveals Sem, SeqSem, UpdateSet, SeqWP, DeleteSet
 
 
-  least predicate VarDeclWitness(st: State, v: Variable, post: iset<State>) {
-    st - {v} in post
+  ghost function UpdateSet(v: Variable, post: iset<State>): iset<State> 
+  {
+    iset st: State | st - {v} in post
+  }
+
+  ghost function DeleteSet(v: Variable, post: iset<State>): iset<State> {
+    iset st: State | exists st' <- post :: st == st' - {v}
   }
 
   least predicate Sem(s: Stmt, st: State, post: iset<State>) {
@@ -15,7 +20,7 @@ module Omni {
     case Assume(e)      => e.IsDefinedOn(st.Keys) && (st.Eval(e) ==> st in post)
     case Seq(ss)        => SeqSem(ss, st, post)
     case Assign(x, v)   => v.IsDefinedOn(st.Keys) && st.Update(x, st.Eval(v)) in post
-    case VarDecl(v, s)  => forall b: Value :: Sem(s, st.Update(v, b), iset st': State | VarDeclWitness(st', v, post))
+    case VarDecl(v, s)  => forall b: Value :: Sem(s, st.Update(v, b), UpdateSet(v, post))
     case Choice(s0, s1) => Sem(s0, st, post) && Sem(s1, st, post)
   }
 
@@ -39,8 +44,7 @@ module Omni {
     ensures Sem(s, st, post')
   {
     match s
-    case VarDecl(v, s) =>
-      assert (iset st': State | VarDeclWitness(st', v, post)) <= (iset st': State | VarDeclWitness(st', v, post'));
+    case VarDecl(v, s) => assert UpdateSet(v, post) <= UpdateSet(v, post');
     case Seq(ss) => SeqSemCons(ss, st, post, post');
     case _ =>
   }
@@ -49,18 +53,9 @@ module Omni {
     requires SeqSem(ss, st, post)
     requires post <= post'
     ensures SeqSem(ss, st, post')
-  {
-
-  }
+  {  }
 
   lemma SemNest(s: Stmt, ss: seq<Stmt>, st: State, post: iset<State>) 
-    requires SeqSem([s] + ss, st, post)
-    ensures Sem(s, st, SeqWP(ss, post))
-  {
-    assert ([s] + ss)[0] == s;
-  }
-
-  lemma SemUnNest(s: Stmt, ss: seq<Stmt>, st: State, post: iset<State>) 
     requires Sem(s, st, SeqWP(ss, post))
     ensures SeqSem([s] + ss, st, post)
   {
@@ -81,34 +76,71 @@ module Omni {
     }
   }
 
-  lemma SeqSemUnNest(ss1: seq<Stmt>, ss2: seq<Stmt>, st: State, post: iset<State>) 
-    requires SeqSem(ss1, st, SeqWP(ss2, post))
-    ensures SeqSem(ss1 + ss2, st, post)
-  {
-    if ss1 == [] {
-      assert [] + ss2 == ss2;
-    } else {
-      assert ([ss1[0]] + (ss1[1..] + ss2))[0] == ss1[0];
-      assert ss1 + ss2 == [ss1[0]] + (ss1[1..] + ss2); 
-    }
-  }
-
   lemma SeqLemma(ss: seq<Stmt>, cont: seq<Stmt>, st: State, post: iset<State>)
     requires Sem(Seq(ss + cont), st, post)
     ensures SeqSem([Seq(ss)] + cont, st, post)
   {
     SeqSemNest(ss, cont, st, post);
-    SemUnNest(Seq(ss), cont, st, post);
+    SemNest(Seq(ss), cont, st, post);
   }
 
-  lemma SeqChoiceLemma(s0: Stmt, s1: Stmt, cont: seq<Stmt>, st: State, post: iset<State>)
-    requires SeqSem([s0] + cont, st, post) 
-    requires SeqSem([s1] + cont, st, post)
-    ensures SeqSem([Choice(s0, s1)] + cont, st, post)
+  lemma FrameLemma(s: Stmt, v: Variable, st: State, post: iset<State>)
+    requires Sem(s, st, post)
+    requires v !in s.FVars()
+    requires v !in s.BVars()
+    ensures Sem(s, st - {v}, DeleteSet(v, post))
   {
-    SemNest(s0, cont, st, post);
-    SemNest(s1, cont, st, post);
-    SemUnNest(Choice(s0, s1), cont, st, post);
+    match s 
+    case Assign(x, e) => e.EvalFVarsLemma(st, st - {v});
+    case Check(e) => e.EvalFVarsLemma(st, st - {v});
+    case Assume(e) =>  e.EvalFVarsLemma(st, st - {v});
+    case Seq(ss) => SeqFrameLemma(ss, v, st, post);
+    case VarDecl(u, s) =>
+      forall c: Value {: trigger}
+        ensures Sem(s, (st - {v}).Update(u, c), UpdateSet(u, DeleteSet(v, post))) { 
+        FrameLemma(s, v, st.Update(u, c), UpdateSet(u, post));
+        assert forall c :: (st - {v}).Update(u, c) == st.Update(u, c) - {v};        
+        SemCons(s, (st - {v}).Update(u, c), DeleteSet(v, UpdateSet(u, post)), UpdateSet(u, DeleteSet(v, post))) by {
+          assert DeleteSet(v, UpdateSet(u, post)) <= UpdateSet(u, DeleteSet(v, post)) by {
+            forall st | st in DeleteSet(v, UpdateSet(u, post)) 
+              ensures st in UpdateSet(u, DeleteSet(v, post)) {
+              assert forall b :: (st - {u}).Update(v, b) == st.Update(v, b) - {u};
+            }
+          }
+        }
+      }
+    case Choice(s0, s1) => FrameLemma(s0, v, st, post); FrameLemma(s1, v, st, post);
   }
 
+  lemma SeqFrameLemma(ss: seq<Stmt>, v: Variable, st: State, post: iset<State>)
+    requires SeqSem(ss, st, post)
+    requires v !in SeqBVars(ss)
+    requires v !in SeqFVars(ss)
+    ensures SeqSem(ss, st - {v}, DeleteSet(v, post))
+  {
+    if ss == [] {
+    } else {
+      assert ([ss[0]] + ss[1..])[0] == ss[0];
+      FrameLemma(ss[0], v, st, SeqWP(ss[1..], post));
+      SemNest(ss[0], ss[1..], st - {v}, DeleteSet(v, post)) by {
+        SemCons(ss[0], st - {v}, DeleteSet(v, SeqWP(ss[1..], post)), SeqWP(ss[1..], DeleteSet(v, post))) by {
+          forall st | st in DeleteSet(v, SeqWP(ss[1..], post)) 
+            ensures SeqSem(ss[1..], st, DeleteSet(v, post)) {
+            var st': State :| st == st' - {v} && SeqSem(ss[1..], st', post);
+            SeqFrameLemma(ss[1..], v, st', post);
+          }
+        }
+      }
+    }
+  }
+
+  lemma SeqFrameLemmaAll(ss: seq<Stmt>, v: Variable, st: State)
+    requires SeqSem(ss, st, AllStates)
+    requires v !in SeqBVars(ss)
+    requires v !in SeqFVars(ss)
+    ensures SeqSem(ss, st - {v}, AllStates)
+  {
+    SeqFrameLemma(ss, v, st, AllStates);
+    SeqSemCons(ss, st - {v}, DeleteSet(v, AllStates), AllStates);
+  }
 }
